Transformation.v
@@ -33,7 +33,7 @@ End Example.
 (* ********************************************************************** *)
 (* * Definition of the transformation *)
 
-(** Grouping transformation 
+(** Grouping transformation
     TODO: add some comments here *)
 
 Record group_tr := make_group_tr {
@@ -48,7 +48,7 @@ Notation make_group_tr' := make_group_tr.
 (** Transformation of paths: π ~ |π| *)
 
 Inductive tr_accesses (gt:group_tr) : accesses -> accesses -> Prop :=
-  | tr_accesses_nil : 
+  | tr_accesses_nil :
       tr_accesses gt nil nil
   | tr_accesses_array : forall π π' i,
       tr_accesses gt π π' ->
@@ -71,7 +71,7 @@ Inductive tr_accesses (gt:group_tr) : accesses -> accesses -> Prop :=
 Inductive tr_val (gt:group_tr) : val -> val -> Prop :=
   | tr_val_error :
       tr_val gt val_error val_error
-  | tr_val_unit : 
+  | tr_val_unit :
       tr_val gt val_unit val_unit
   | tr_val_bool : forall b,
       tr_val gt (val_bool b) (val_bool b)
@@ -84,20 +84,20 @@ Inductive tr_val (gt:group_tr) : val -> val -> Prop :=
       tr_val gt (val_abstract_ptr l π) (val_abstract_ptr l π')
   | tr_val_array : forall a a',
       length a = length a' ->
-      (forall i, 
-        index a i -> 
-        tr_val gt a[i] a'[i]) -> 
+      (forall i,
+        index a i ->
+        tr_val gt a[i] a'[i]) ->
       tr_val gt (val_array a) (val_array a')
   | tr_val_struct_group : forall Ts Tsg s s' fg fs sg,
       gt = make_group_tr Ts fs Tsg fg ->
-      fs \c dom s ->  
+      fs \c dom s ->
       fg \notindom s ->
       dom s' = (dom s \- fs) \u \{fg} ->
       dom sg = fs ->
       (forall f,
         f \indom sg ->
         tr_val gt s[f] sg[f]) ->
-      (forall f,       
+      (forall f,
         f \notin fs ->
         f \indom s ->
         tr_val gt s[f] s'[f]) ->
@@ -146,19 +146,19 @@ Inductive tr_trm (gt:group_tr) : trm -> trm -> Prop :=
       r = trm_app a1 ((trm_app a2 (p'::nil))::nil) ->
       tr_trm gt (trm_app (prim_struct_access s f) (p::nil)) r
   | tr_trm_struct_access_other : forall s p p' T f r,
-      tr_trm gt p p' -> 
+      tr_trm gt p p' ->
       s = group_tr_struct_name gt ->
-      (T <> s \/ f \notin (group_tr_fields gt)) ->       
+      (T <> s \/ f \notin (group_tr_fields gt)) ->
       r = (trm_app (prim_struct_access T f) (p'::nil)) ->
       tr_trm gt (trm_app (prim_struct_access T f) (p::nil)) r
   (* Args *)
   | tr_trm_args1 : forall op t1 t1',
       ~ is_prim_struct_access op ->
-      tr_trm gt t1 t1' -> 
+      tr_trm gt t1 t1' ->
       tr_trm gt (trm_app op (t1::nil)) (trm_app op (t1'::nil))
   | tr_trm_args2 : forall op t1 t1' t2 t2',
-      tr_trm gt t1 t1' -> 
-      tr_trm gt t2 t2' -> 
+      tr_trm gt t1 t1' ->
+      tr_trm gt t2 t2' ->
       tr_trm gt (trm_app op (t1::t2::nil)) (trm_app op (t1'::t2'::nil)).
 
 
@@ -170,9 +170,9 @@ Inductive tr_trm (gt:group_tr) : trm -> trm -> Prop :=
     A more direct definition for the domain equality is
     [forall x, fresh x S <-> fresh x S'].
 
-    An alternative, is to impose the stack to have the same 
+    An alternative, is to impose the stack to have the same
     structure, with [tr_stack S S' := LibList.Forall2 tr_stack_item S S']
-    with [Inductive tr_stack_item : 
+    with [Inductive tr_stack_item :
             | tr_stack_item_intro : tr_val v1 v2 -> tr_stack_item (x,v1) (x,v2).]
     Then, by constructions, the stacks have the same domains.
     I would probably recommand this version, and proving as derived lemma
@@ -227,7 +227,7 @@ Qed.
 
 Hint Resolve index_of_index_length'.
 
-Hint Constructors red tr_trm tr_val tr_accesses tr_state tr_stack 
+Hint Constructors red tr_trm tr_val tr_accesses tr_state tr_stack
                   read_accesses write_accesses.
 
 
@@ -248,20 +248,20 @@ Proof.
     inverts H11; tryfalse. }
   { inverts H2; repeat fequals*;
     inverts H0; tryfalse. }
-Qed. 
+Qed.
 
 Theorem functional_tr_val : forall gt v v1 v2,
   tr_val gt v v1 ->
   tr_val gt v v2 ->
   v1 = v2.
 Proof using.
-  introv H1 H2. gen v2. induction H1; intros; 
+  introv H1 H2. gen v2. induction H1; intros;
   inverts_head tr_val; try solve [ fequals* ].
   { fequals. applys* functional_tr_accesses. }
   { fequals. applys* eq_of_extens. math. }
-  { (*subst. inverts_head make_group_tr'. fequals. 
+  { (*subst. inverts_head make_group_tr'. fequals.
     applys* map_ext. rew_set in *. intuition. {  } intuition. auto.
-    { admit. } 
+    { admit. }
     { admit. } }
   { subst. simpls. contradiction.*) admit. }
   { admit. }
@@ -312,7 +312,7 @@ Proof.
      not that from TLC. I changed that by remove "open scope list_scope". *)
   (* TODO: look at new proof using [rew_list] *)
   introv Ha1 Ha2. gen π2 π2'. induction Ha1; intros;
-    rew_list in *; eauto. 
+    rew_list in *; eauto.
   (* old proof deprecated:
   introv Ha1 Ha2. gen π2 π2'. induction Ha1; intros;
   try solve [ subst ; forwards Ha': IHHa1 Ha2 ;
@@ -379,8 +379,8 @@ Lemma neq_tr : forall gt v1 v2 v1' v2',
 Proof.
 Admitted.
 
-Axiom not_tr_val_error : forall gt v1 v2, 
-  tr_val gt v1 v2 -> 
+Axiom not_tr_val_error : forall gt v1 v2,
+  tr_val gt v1 v2 ->
   ~ is_error v2.
 
 
@@ -426,15 +426,15 @@ Ltac set_prove_show :=
 (** Auxiliary set results *)
 
 
-Lemma in_union : forall A (x:A) (S1 S2:set A), 
-        (x \in S1) \/ (x \in S2) -> 
+Lemma in_union : forall A (x:A) (S1 S2:set A),
+        (x \in S1) \/ (x \in S2) ->
         x \in (S1 \u S2).
 Proof using. set_prove. Qed.
 
 
 Lemma in_setminus : forall A (x:A) (S1 S2: set A),
-        x \in S1 -> 
-        x \notin S2 -> 
+        x \in S1 ->
+        x \notin S2 ->
         x \in (S1 \- S2).
 Proof using. set_prove. Qed.
 
@@ -502,7 +502,7 @@ Lemma index_of_index_update_at_index : forall A B `{Inhab B} (m:map A B) (i j:A)
   index m i ->
   index m j.
 Proof using.
-  introv IB H1 H2. rewrite index_update_eq in H1. destruct H1; subst*. 
+  introv IB H1 H2. rewrite index_update_eq in H1. destruct H1; subst*.
   rewrite index_eq_indom in *. auto.
   (* forwards*: indom_of_indom_update_at_indom. *)
 Qed.
@@ -546,51 +546,51 @@ Lemma tr_read_accesses : forall gt v π v' π' w,
   /\  read_accesses v' π' w').
 Proof.
   introv Hv Ha HR. gen gt v' π'. induction HR; intros.
-  { (* nil *) 
-    inverts Ha. exists* v'. } 
+  { (* nil *)
+    inverts Ha. exists* v'. }
   { (* array_access *)
     inverts Ha as Ha. inverts Hv as Hl Htr.
-    forwards Htra: Htr H. 
+    forwards Htra: Htr H.
     forwards (w'&Hw'&Hπ'): IHHR Htra Ha.
     exists* w'. }
-  { (* struct_access *) 
-    inverts Ha as; inverts Hv as; 
+  { (* struct_access *)
+    inverts Ha as; inverts Hv as;
     try solve [ intros ; false ].
-    { (* one of the fields to group *) 
+    { (* one of the fields to group *)
       introv HD1 Hgt HD2 HD3 Hsg Hfs HB Ha Hin.
 (*  sets_eq Gtn: (group_tr_struct_name gt).
 subst gt. simpls.*)
       rewrite* Hgt in Hin. simpls.
       forwards Hsf: Hsg Hin.
-      forwards Heq: read_of_binds H. 
+      forwards Heq: read_of_binds H.
       subst_hyp Heq.
       forwards (w'&Hw'&HR'): IHHR Hsf Ha.
       exists* w'. splits*.
-      constructors*; rewrite Hgt; simpls*. 
+      constructors*; rewrite Hgt; simpls*.
       constructors*. applys* binds_of_indom_read. }
-    { (* struct transformed but another field *) 
+    { (* struct transformed but another field *)
       introv HD1 HD2 HD3 Hsg Hfs HB Ha Hor.
       inverts Hor as Hf; simpl in Hf; tryfalse.
       forwards Hf': indom_of_binds H. typeclass.
       forwards Hsf: Hfs Hf Hf'.
-      forwards Hv1: read_of_binds H. 
+      forwards Hv1: read_of_binds H.
       subst_hyp Hv1.
       forwards (w'&Hw'&HR'): IHHR Hsf Ha.
-      exists w'. splits*. constructors*. 
+      exists w'. splits*. constructors*.
       applys* binds_of_indom_read.
       rewrite HD3. rew_set*.
-(*   left*. applys* in_union. 
+(*   left*. applys* in_union.
       left. applys* in_setminus. *) }
     { (* another struct *)
-      intros Hn HD Hfs Ha Hor. 
+      intros Hn HD Hfs Ha Hor.
       forwards Hidx: index_of_binds H. typeclass.
-      forwards Hsf: Hfs Hidx. 
+      forwards Hsf: Hfs Hidx.
       forwards Heq: read_of_binds H.
-      subst_hyp Heq. 
+      subst_hyp Heq.
       forwards (w'&Hw'&HR'): IHHR Hsf Ha.
-      exists w'. splits*. constructors*. 
+      exists w'. splits*. constructors*.
       applys* binds_of_indom_read.
-      rewrite <- HD. 
+      rewrite <- HD.
       rewrite* <- index_eq_indom. } }
 Qed.
 
@@ -614,11 +614,11 @@ Proof.
     splits; constructors*.
     { (* val_array under tr *)
       rewrite H0. repeat rewrite* length_update. }
-    { (* write_accesses of transformed array *) 
-      introv Hi0. rewrite read_update_case. 
+    { (* write_accesses of transformed array *)
+      introv Hi0. rewrite read_update_case.
       { (* HERE, should do [case_if as C] *) case_if*; subst_hyp H0.
         { subst_hyp C. rewrites* LibListZ.read_update_same. }
-        { forwards: index_of_update_neq' Hi0 C. 
+        { forwards: index_of_update_neq' Hi0 C.
           rewrites* LibListZ.read_update_neq. } }
       { rewrite index_eq_index_length in *.
         rewrite H0 in Hi0. rewrite length_update in Hi0.
@@ -626,18 +626,18 @@ Proof.
   { (* struct_access *)
     inverts Ha as; inverts Hv1 as;
     try solve [ intros ; false ].
-    { (* one of the fields to group *) 
+    { (* one of the fields to group *)
       introv HD1 Hgt HD2 HD3 Hsg Hfs HB Ha Hin.
       rewrite* Hgt in Hin. simpls.
       forwards Hsf: Hsg Hin.
-      forwards Heq: read_of_binds H. 
+      forwards Heq: read_of_binds H.
       subst_hyp Heq.
       forwards (v2'&Hv2'&HW'): IHHW Hsf Hw Ha.
       remember (group_tr_struct_name gt) as T.
       exists (val_struct T s'[fg:=(val_struct Tsg sg[f:=v2'])]).
       splits.
-      { substs. 
-        applys tr_val_struct_group (sg[f:=v2']); try reflexivity; 
+      { substs.
+        applys tr_val_struct_group (sg[f:=v2']); try reflexivity;
         repeat rewrite dom_update_at_indom; try typeclass;
         try solve [ applys* in_subset ].
         (*Ltac rew_dom_at_core tt := repeat rewrite dom_update_at_indom.
@@ -645,17 +645,17 @@ Proof.
         Tactic Notation "rew_dom_at" "*" := rew_dom_at; auto_star.*)
         { forwards*: indom_of_binds HB. }
         { introv HD4. repeat rewrite read_update. case_if*. }
-        { introv HD4 HD5. repeat rewrite read_update. 
+        { introv HD4 HD5. repeat rewrite read_update.
           repeat case_if*; subst; contradiction. }
         { applys* binds_update_same. } }
       { constructors*; subst_hyp Hgt; simpls*.
         constructors*. applys* binds_of_indom_read. } }
-    { (* struct transformed but another field *) 
-      introv HD1 HD2 HD3 Hsg Hfs HB Ha Hor. 
+    { (* struct transformed but another field *)
+      introv HD1 HD2 HD3 Hsg Hfs HB Ha Hor.
       inverts Hor as Hf; simpl in Hf; tryfalse.
       forwards Hf': indom_of_binds H. typeclass.
       forwards Hsf: Hfs Hf Hf'.
-      forwards Hv1: read_of_binds H. 
+      forwards Hv1: read_of_binds H.
       subst_hyp Hv1.
       forwards (v2'&Hv2'&HW'): IHHW Hsf Hw Ha.
       exists (val_struct T s'[f:=v2']). splits.
@@ -663,7 +663,7 @@ Proof.
         try solve [ rewrite* dom_update_at_indom ].
         { repeat rewrite* dom_update_at_indom.
           rewrite HD3. applys* in_union. left.
-          applys* in_setminus. }        
+          applys* in_setminus. }
         { introv Hf0. rewrite read_update. case_if*.
           forwards: in_notin_neq Hf0 Hf. false. }
         { introv HD4 HD5. repeat rewrite read_update.
@@ -676,9 +676,9 @@ Proof.
     { (* another struct *)
       intros Hn HD Hfs Ha Hor.
       forwards Hidx: index_of_binds H. typeclass.
-      forwards Hsf: Hfs Hidx. 
+      forwards Hsf: Hfs Hidx.
       forwards Heq: read_of_binds H.
-      subst_hyp Heq. 
+      subst_hyp Heq.
       forwards (v2'&Hv2'&HW'): IHHW Hsf Hw Ha.
       exists (val_struct T s'[f:=v2']). splits.
       { constructors*; subst_hyp H0.
@@ -688,7 +688,7 @@ Proof.
           rewrites* dom_update_at_indom. }
         { introv Hif0. rewrite read_update. case_if*.
           { subst_hyp C. rewrite* read_update_same. }
-          { rewrite* read_update_neq. 
+          { rewrite* read_update_neq.
             forwards Hif0': index_of_index_update_neq Hif0 C. auto.
             forwards*: Hfs Hif0'. } } }
       { constructors*. applys* binds_of_indom_read.
@@ -702,14 +702,14 @@ Qed.
 
 Axiom isTrue_var_eq : forall A (v1 v2:A), v1 = v2 -> isTrue (v1 = v2) = true.
 
-Axiom isTrue_var_neq : forall A (v1 v2:A), v1 <> v2 -> isTrue (v1 = v2) = false. 
+Axiom isTrue_var_neq : forall A (v1 v2:A), v1 <> v2 -> isTrue (v1 = v2) = false.
 
 Theorem red_tr: forall gt t t' v S S' m1 m1' m2,
   tr_trm gt t t' ->
   tr_stack gt S S' ->
   tr_state gt m1 m1' ->
-  red S m1 t m2 v -> 
-  ~ is_error v -> 
+  red S m1 t m2 v ->
+  ~ is_error v ->
   exists v' m2',
       tr_val gt v v'
   /\  tr_state gt m2 m2'
@@ -718,17 +718,17 @@ Proof.
   introv Ht HS Hm1 HR He. gen t' S' m1'. induction HR; intros;
   try solve [ forwards*: He; unfolds* ].
   { (* var *)
-    inverts Ht. inverts HS. 
+    inverts Ht. inverts HS.
     forwards: H1 H. inverts H2. exists* x0 m1'. }
   { (* val *)
     inverts Ht. exists* v' m1'. }
   { (* if *)
-    inverts Ht as Hb HTrue HFalse. 
+    inverts Ht as Hb HTrue HFalse.
     forwards (v'&m2'&Hv'&Hm2'&HR3): IHHR1 Hb HS Hm1.
     introv HN. inverts HN.
     inverts* Hv'.
-    forwards* (vr'&m3'&Hvr'&Hm3'&HR4): IHHR2 HS Hm2'. 2: 
-    exists* vr' m3'. case_if*. } 
+    forwards* (vr'&m3'&Hvr'&Hm3'&HR4): IHHR2 HS Hm2'. 2:
+    exists* vr' m3'. case_if*. }
   { (* let *)
     inverts Ht as Ht1 Ht2.
     forwards* (v'&m2'&Hv'&Hm2'&HR3): IHHR1 Ht1 HS Hm1.
@@ -739,14 +739,14 @@ Proof.
   { (* binop *)
     inverts Ht as Ht1 Ht2.
     inverts Ht1 as Ht1. inverts Ht2 as Ht2.
-    inverts H; 
+    inverts H;
     try solve [ exists __ m1'; splits*;
-    inverts Ht1; inverts Ht2; 
+    inverts Ht1; inverts Ht2;
     repeat constructors* ].
     (* equality case *)
     exists (val_bool (isTrue (v' = v'0))) m1'.
     splits*.
-    { tests C: (v1 = v2). 
+    { tests C: (v1 = v2).
       { forwards: functional_tr_val Ht1 Ht2. subst.
         repeat rewrite* isTrue_var_eq. }
       { forwards*: neq_tr.
@@ -759,9 +759,9 @@ Proof.
     subst_hyp H. inverts Hp as Hp. inverts Hp.
     forwards: read_of_binds Hb. subst_hyp H.
     forwards (w'&Hw'&Ha'): tr_read_accesses Htrml H2 Ha.
-    exists w' m1'. splits*. 
+    exists w' m1'. splits*.
     constructors*. constructors*.
-    applys* binds_of_indom_read. 
+    applys* binds_of_indom_read.
     rewrite <- HD at 1.
     forwards*: indom_of_binds Hb. }
   { (* set *)
@@ -769,40 +769,40 @@ Proof.
     inverts H2 as Hb HW. forwards Hi: index_of_binds Hb.
     typeclass. forwards Htrml: Htrm Hi. subst_hyp H.
     inverts Hp as Hp. inverts Hp as Ha.
-    subst_hyp H0. inverts Ht as Hv. 
+    subst_hyp H0. inverts Ht as Hv.
     forwards Heq: read_of_binds Hb. subst_hyp Heq.
     forwards (w'&Hw'&HW'): tr_write_accesses Htrml Hv Ha HW.
     exists val_unit m1'[l:=w']. splits*.
-    { constructors. 
+    { constructors.
       { rewrite index_eq_indom in Hi.
         forwards* HDm1: dom_update_at_indom Hi.
         rewrite HD in Hi at 1.
         forwards* HDm1': dom_update_at_indom Hi.
         rewrite* HDm1. rewrite* HDm1'. }
       { introv Hi'. do 2 rewrites read_update.
-        case_if*. 
+        case_if*.
         forwards* Hi'': index_of_index_update_neq Hi' C. } }
     { constructors*. applys* not_tr_val_error.
       constructors*. applys* binds_of_indom_read.
       rewrite <- HD at 1. forwards*: indom_of_binds Hb. } }
-  { (* new *) 
-    inverts Ht as _ Ht. inverts Ht as Hv. 
+  { (* new *)
+    inverts Ht as _ Ht. inverts Ht as Hv.
     inverts Hm1 as HD Htrm.
     subst_hyp H1.
     exists (val_abstract_ptr l0 nil) m1'[l0:=v'].
     splits*.
-    { constructors. 
-      { unfold state. repeat rewrite dom_update. 
+    { constructors.
+      { unfold state. repeat rewrite dom_update.
         applys* union_eq.  }
       { introv Hi. rewrite read_update. case_if*.
         { subst_hyp C. rewrite* read_update_same. }
-        { rewrite* read_update_neq. 
+        { rewrite* read_update_neq.
           forwards* Hi': index_of_index_update_neq Hi C. } } }
     { constructors*. rewrite* <- HD. } }
-  { (* struct_access *) 
+  { (* struct_access *)
     inverts Ht as; inverts Hm1 as HD Htrm.
     { (* accessing grouped field *)
-      introv Ht Hf. subst. 
+      introv Ht Hf. subst.
       inverts Ht as Hv. inverts Hv as Ha.
       remember (group_tr_struct_name gt) as Ts.
       remember (group_tr_new_struct_name gt) as Tsg.
@@ -814,20 +814,20 @@ Proof.
       { constructors. applys* tr_accesses_app. subst*. }
       { subst. applys* red_args_1. applys* red_struct_access.
         fequals*. rew_list*. (* TODO: was: rewrite* <- List.app_assoc. *) } }
-    { (* accessing another field *) 
+    { (* accessing another field *)
       introv Ht Hor. subst. inverts Ht as Hv. inverts Hv as Ha.
       exists (val_abstract_ptr l (π'++(access_field T f :: nil))) m1'.
-      splits; constructors*. applys* tr_accesses_app. } 
+      splits; constructors*. applys* tr_accesses_app. }
     { introv HN. forwards*: HN. } }
   { (* array_access *)
-    inverts Ht as Ht Hti. subst. 
+    inverts Ht as Ht Hti. subst.
     inverts Ht as Hv. inverts Hv as Ha.
     inverts Hti as Hv. inverts Hv.
     inverts Hm1 as HD Htrm.
-    exists (val_abstract_ptr l (π'++(access_array i::nil))) m1'. 
+    exists (val_abstract_ptr l (π'++(access_array i::nil))) m1'.
     splits; constructors*. applys* tr_accesses_app. }
-  { (* args_1 *) 
-    inverts Ht; forwards* (v'&m2'&Hv'&Hm2'&HR'): IHHR1; 
+  { (* args_1 *)
+    inverts Ht; forwards* (v'&m2'&Hv'&Hm2'&HR'): IHHR1;
     forwards*: red_app_not_is_error HR2 He;
     forwards* (v''&m3'&Hv''&Hm3'&HR''): IHHR2;
     exists v'' m3'; splits*;
@@ -835,16 +835,16 @@ Proof.
     (* remaining cases are structs *)
     inverts HR''.
     { inverts H10. }
-    { applys* red_args_1. applys* red_args_1. 
+    { applys* red_args_1. applys* red_args_1.
       apply not_is_val_tr with (gt:=gt) (t1:=t1); auto. }
     { forwards HN: not_is_error_tr He Hv''. forwards*: HN. unfolds*. }
     { forwards HN: not_is_error_tr He Hv''. forwards*: HN. unfolds*. } }
-  { (* args_2 *) 
+  { (* args_2 *)
     inverts Ht as Ht1 Ht2.
     forwards* (v'&m2'&Hv'&Hm2'&HR'): IHHR1.
     forwards*: red_app_not_is_error_2 HR2 He.
-    forwards* (v''&m3'&Hv''&Hm3'&HR''): IHHR2. 
-    exists v'' m3'. splits*. 
+    forwards* (v''&m3'&Hv''&Hm3'&HR''): IHHR2.
+    exists v'' m3'. splits*.
     inverts Ht1. applys* red_args_2.
     applys* not_is_val_tr. }
 Qed.
